### Q1

We have
$$
J(\theta)=-\sum^m_{i=1}y_ilog(h_\theta(x_i))+(1-y_i)log(1-h_\theta(x_i))
$$
So the verify process is as follow:

First:
$$
\begin{aligned}\frac{\partial h_\theta(x_i)}{\partial\theta}&=
\frac{\partial(\frac{1}{1+exp(-\theta^Tx)})}{\partial\theta}\\
&=\frac{1+exp(-\theta^Tx)-exp(-\theta^Tx)}{(1+exp(-\theta^Tx))^2}*\frac{\partial(-\theta^Tx)}{\partial\theta}\\
&=\frac{exp(-\theta^Tx)*x}{(1+exp(-\theta^Tx))^2}\\
&=h_\theta(x)(1-h_\theta(x))*x
\end{aligned}
$$
Then:
$$
\begin{aligned}
\frac{\partial J(\theta)}{\partial \theta}&=-\sum^m_{i=1}(y_i*\frac{1}{h_\theta(x_i)}*\frac{\partial h_\theta(x_i)}{\theta}-(1-y_i)*\frac{1}{1-h_\theta(x_i)}* \frac{\partial h_\theta(x_i)}{\partial \theta}      )\\
&=-\sum^m_{i=1}(y_i*\frac{1}{h_\theta(x_i)}-(1-y_i)*\frac{1}{1-h_\theta(x_i)}      )*\frac{\partial h_\theta(x_i)}{\theta}\\
&=-\sum^m_{i=1}(y_i*\frac{1}{h_\theta(x_i)}-(1-y_i)*\frac{1}{1-h_\theta(x_i)}      )*h_\theta(x_i)(1-h_\theta(x_i))*x_i\\
&=-\sum^m_{i=1}(y_i*(1-h_\theta(x_i))-(1-y_i)* h_\theta(x_i)     )*x_i\\
&=-\sum^m_{i=1}(y_i-h_\theta(x_i))*x_i
\end{aligned}
$$
